README.md
@@ -5,7 +5,7 @@ Current Design of DateTime API
 ## How to execute the test example
 
 ```
-dafny build --target:cs TestLocalDateTime.dfy LocalDateTimeImpl.cs
+dafny build TestLocalDateTime.dfy --target:cs TestLocalDateTime.dfy LocalDateTimeImpl.cs --standard-libraries
 
 ./TestLocalDateTime
 ```
